# Functions - Pg. 22, Sec 1, 2, 4, 5, 6b, 7 & 8b

## Sec 1: Solve $$\displaylines{f(x)=2-3x\\}$$
### a) f(2)
$$\displaylines{f(2)=2-3*2\\2-6\\=-4}$$
### b) f(0)
$$\displaylines{f(2)=2-3*0\\=2}$$
### c) f(-4)
$$\displaylines{f(2)=2-3*-4\\2+12\\=14}$$
### d) f(1/2)
$$\displaylines{f(2)=2-3*\frac{1}{2}\\\frac{4}{2}-\frac{3}{2}\\=\frac{1}{2}}$$
### e) f(a)
$$\displaylines{f(2)=2-3a\\=2-3a}$$
### f) f(3b)
$$\displaylines{f(2)=2-3*3b\\=2-9b}$$


## Sec 2: The Graphs of y = f(x) & y = g(x)
![[Pasted image 20240909150903.png]]
Evaluate each function
### $$\displaylines{f(1) = 2}$$
### $$\displaylines{g(-2)}=4$$
### $$\displaylines{f(4) - g(-2) \\ =(-1) - 4 \\=(-5)}$$
### $$\displaylines{f(x)=-3, x = -3,-4}$$
## Sec 4: Evaluate f(-1), f(3), & f(1.5) for
### a) $$f(x)=(x-2)^2-1$$
$$\displaylines{f(-1) = (-1-2)^2-1\\=-3^2-1\\=9-1\\=8}$$
$$\displaylines{f(3) = (3-2)^2-1\\=1^2-1\\=1-1\\=0}$$
$$\displaylines{f(1.5) = (1.5-2)^2-1\\=-0.5^2-1\\=0.25-1\\=-0.75}$$

### b) $$\displaylines{f(x)=2+3x-4x^2}$$
$$\displaylines{f(-1) = 2 + 3(-1)-4(-1)^2\\2-3-4\\=(-5)}$$$$\displaylines{f(3) = 2 + 3(3)-4(3)^2\\2+9-36\\=(-25)}$$$$\displaylines{f(1.5) = 2 + 3(1.5)-4(1.5)^2\\2+4.5-9\\=(-2.5)}$$
## Sec 5: Evaluate 4 cases of $$f(x) = \frac{1}{2x}$$
### a) 
$$\displaylines{f(-3) = \frac{1}{2(-3)}\\=-\left( \frac{1}{6} \right)}$$
### b) 
$$\displaylines{f(0) = \frac{1}{2(0)}\\=\frac{1}{0}\\ = \pm\infty }$$
or undefined if you are no fun...
### c) $$\displaylines{f(1) - f(3) = \frac{1}{2(1)} - \frac{1}{2(3)} \\ = \frac{1}{2} - \frac{1}{6}\\=\frac{3}{6}-\frac{1}{6}\\ = \frac{2}{6}\\= \frac{1}{3}}$$

### d) $$\displaylines{f\left( \frac{1}{4} \right) + f\left( \frac{3}{4} \right) = \frac{1}{2\left( \frac{1}{4} \right)} + \frac{1}{2\left( \frac{3}{4} \right)}\\=\frac{1}{\frac{1}{2}}+\frac{1}{\frac{3}{2}}\\=\frac{2}{1} + \frac{2}{3}\\=\frac{6}{3}+\frac{2}{3}\\=\frac{8}{3}}$$

## Sec 6b
The graph of y=f(x) is not shown on the right (11pm right now), so just evaluate *even more*.
### a) 
$$f(3)=4$$
### b) 
$$f(5)=2$$
### c) 
$$f(5-3)=f(2)=5$$
### d) 
$$f(5)-f(3)=2-4=(-2)$$


## Sec 7 $$h(x) = 2x - 5$$
### a) 
$$h(a) = 2a-5$$
### b) 
$$\displaylines{h(b+1) = 2(b+1)-5\\2b+2-5\\=2b-3}$$
### c) 
$$\displaylines{h(3c-1) = 2(3c-1)-5\\6c-2-5\\=6c-7}$$
### d) 
$$\displaylines{h(2-5x) = 2(2-5x)-5\\4-10x-5\\=-10x+4-5\\=-10x-1}$$

## Sec 8b $$g(t) = 3t + 5$$
### a) 
$$g(0)=3(0)+5=5$$
### b) 
$$g(3)=3(3)+5=9+5=14$$
### c) 
$$\displaylines{g(1)-g(0)\\=3(1)+5-3(0)+5\\=8-5\\=3}$$
### d) 
$$\displaylines{g(2)-g(1)\\=3(2)+5-3(1)+5\\=11-8\\=3}$$
### e)
$$\displaylines{g(1001)-g(1000)\\=3(1001)+5-3(1000)+5\\=3008-3005\\=3}$$
### f)
$$\displaylines{g(a+1)-g(a)\\=3(a+1)+5-3(a)+5\\=3a+3+5-3a+5\\=3a-3a+8-5\\=3}$$